# baseURI: https://w3id.org/fog
# prefix: fog

@prefix : <https://w3id.org/fog#> .
@prefix cc: <http://creativecommons.org/ns#> .
@prefix dbp: <http://dbpedia.org/property/> .
@prefix dbr: <http://dbpedia.org/resource/> .
@prefix dcterms: <http://purl.org/dc/terms/> .
@prefix foaf: <http://xmlns.com/foaf/0.1/> .
@prefix fog: <https://w3id.org/fog#> .
@prefix geo: <http://www.opengis.net/ont/geosparql#> .
@prefix omg: <https://w3id.org/omg#> .
@prefix owl: <http://www.w3.org/2002/07/owl#> .
@prefix rdf: <http://www.w3.org/1999/02/22-rdf-syntax-ns#> .
@prefix rdfs: <http://www.w3.org/2000/01/rdf-schema#> .
@prefix vann: <http://purl.org/vocab/vann/> .
@prefix voaf: <http://purl.org/vocommons/voaf#> .
@prefix wd: <https://www.wikidata.org/entity/> .
@prefix xsd: <http://www.w3.org/2001/XMLSchema#> .

<https://w3id.org/fog>
  rdf:type voaf:Vocabulary ;
  rdf:type owl:Ontology ;
  cc:license <https://creativecommons.org/licenses/by/4.0/> ;
  dcterms:creator <https://www.researchgate.net/profile/Anna_Wagner13> ;
  dcterms:creator <https://www.researchgate.net/profile/Mathias_Bonduel> ;
  dcterms:creator <https://www.researchgate.net/profile/Pieter_Pauwels> ;
  dcterms:description """The File Ontology for Geometry formats (FOG) describes meaningful relations towards geometry snippets in RDF literals, geometry files on relative or absolute URLs and ontology-based geometry descriptions. The defined properties in this ontology are related towards each other and additional metadata is provided, such as file extension and related specifications/sources (incl. entries in dbpedia and Wikidata). 

The initial version of the ontology (v0.0.1) was documented in:

Bonduel, M., Wagner, A., Pauwels, P., Vergauwen, M., & Klein, R. (2019). Including Widespread Geometry Formats in Semantic Graphs Using RDF Literals. In Proceedings of the European Conference on Computing in Construction (EC3 2019). Chania, Greece."""@en ;
  dcterms:issued "2018-12-03"^^xsd:date ;
  dcterms:modified "2020-01-14"^^xsd:date ;
  dcterms:title "FOG: File Ontology for Geometry formats"@en ;
  vann:example "https://madsholten.github.io/sparql-visualizer/?file=https://raw.githubusercontent.com/mathib/fog-ontology/master/examples/fog-demo.json"^^xsd:anyURI ;
  vann:example "https://raw.githubusercontent.com/mathib/fog-ontology/master/examples/sample_abox_columns.ttl"^^xsd:anyURI ;
  vann:example "https://raw.githubusercontent.com/mathib/fog-ontology/master/examples/sample_abox_columns_dummy.ttl"^^xsd:anyURI ;
  vann:example "https://raw.githubusercontent.com/mathib/fog-ontology/master/examples/sample_abox_snk_contractor.ttl" ;
  vann:example "https://raw.githubusercontent.com/mathib/fog-ontology/master/examples/sample_abox_snk_inspector.ttl" ;
  vann:preferredNamespacePrefix "fog" ;
  vann:preferredNamespaceUri "https://w3id.org/fog#" ;
  rdfs:comment """- Version 0.0.4:
* added subproperties of omg:hasReferencedGeometryId: OBJ, Revit, Rhino, IFC
- Version 0.0.3: 
* added datatype properties: Nexus, LAS
* added subproperties for fog:asPcd: ascii and binary
- Version 0.0.2: 
* updated definitions of certain properties
* adjusted typos
* added datatype properties for: Rhino, Revit, IFC, STEP APs, IGES
* added object properties for: 3DMO, ifcOWL, geojson-ld
* completed ontology metadata
- Version 0.0.1: initial version"""@en ;
  owl:versionInfo "0.0.4" ;
.
fog:
  rdf:type owl:Ontology ;
.
fog:ReferencedContent
  rdf:type owl:Class ;
  rdfs:comment "Referenced content of the following geometry descriptions: glTF and OBJ. It contains exactly one link to a texture, separate binary glTF geometry or a OBJ material that is referenced by the main file (resp. .gltf and .obj). The name of the referenced file, as stored in the main file, is connected via a rdfs:label node"@en ;
  rdfs:isDefinedBy fog: ;
  rdfs:label "Referenced content"@en ;
.
fog:as3dmo
  rdf:type owl:FunctionalProperty ;
  rdf:type owl:ObjectProperty ;
  rdfs:comment "The object relation pointing to a RDF-based geometry description following the 3DMO ontology. It is strongly adviced to use the more specific subproperty (fog:as3dmo_v1.1)"@en ;
  rdfs:isDefinedBy fog: ;
  rdfs:label "as 3DMO ontology"@en ;
  rdfs:seeAlso <https://web.archive.org/web/20180831114523/http://3dontology.org/3d.ttl> ;
  rdfs:subPropertyOf omg:hasComplexGeometryDescription ;
.
<https://w3id.org/fog#as3dmo_v1.1>
  rdf:type owl:FunctionalProperty ;
  rdf:type owl:ObjectProperty ;
  rdfs:comment "The object relation pointing to a RDF-based geometry description following the 3DMO ontology version 1.1. It should be connected to the topnode of the geometry description"@en ;
  rdfs:isDefinedBy fog: ;
  rdfs:label "as 3DMO v1.1 ontology"@en ;
  rdfs:seeAlso <https://web.archive.org/web/20180831114523/http://3dontology.org/3d.ttl> ;
  rdfs:subPropertyOf fog:as3dmo ;
.
fog:asCollada
  rdf:type owl:DatatypeProperty ;
  rdf:type owl:FunctionalProperty ;
  rdfs:comment "The datatype relation pointing to a geometry description following the open COLLADA format from the Khronos Group. The format consists of a single .dae file (text-based). It is strongly adviced to use the more specific subproperties (e.g. fog:asCollada_v1.4.1)."@en ;
  rdfs:isDefinedBy fog: ;
  rdfs:label "as COLLADA format"@en ;
  rdfs:seeAlso dbr:COLLADA ;
  rdfs:seeAlso <https://www.iana.org/assignments/media-types/model/vnd.collada+xml> ;
  rdfs:seeAlso wd:Q603967 ;
  rdfs:subPropertyOf omg:hasSimpleGeometryDescription ;
.
<https://w3id.org/fog#asCollada_v1.4.1>
  rdf:type owl:DatatypeProperty ;
  rdf:type owl:FunctionalProperty ;
  dbp:extension ".dae" ;
  rdfs:comment "The datatype relation pointing to a geometry description following the open COLLADA v1.4.1 format from the Khronos Group. It consists of a single .dae file (text-based)."@en ;
  rdfs:isDefinedBy fog: ;
  rdfs:label "as COLLADA v1.4.1 format (.dae)"@en ;
  rdfs:seeAlso <https://www.khronos.org/files/collada_spec_1_4.pdf> ;
  rdfs:seeAlso wd:Q28975679 ;
  rdfs:subPropertyOf fog:asCollada ;
.
<https://w3id.org/fog#asCollada_v1.5.0>
  rdf:type owl:DatatypeProperty ;
  rdf:type owl:FunctionalProperty ;
  dbp:extension ".dae" ;
  rdfs:comment "The datatype relation pointing to a geometry description following the open COLLADA v1.5.0 format from the Khronos Group. It consists of a single .dae file (text-based)."@en ;
  rdfs:label "as COLLADA v1.5.0 format (.dae)"@en ;
  rdfs:seeAlso <https://www.khronos.org/files/collada_spec_1_5.pdf> ;
  rdfs:subPropertyOf fog:asCollada ;
.
fog:asDwg
  rdf:type owl:DatatypeProperty ;
  rdf:type owl:FunctionalProperty ;
  rdfs:comment "The datatype relation pointing to a geometry description following the proprietary DWG format from Autodesk. The Open Design Alliance created a 'specification for .dwg files' that is publicly available. The format consists of a single .dwg file (binary). It is strongly adviced to use the more specific subproperties (e.g. fog:asDwg_v2018)."@en ;
  rdfs:label "as DWG format"@en ;
  rdfs:seeAlso <http://dbpedia.org/resource/.dwg> ;
  rdfs:seeAlso <https://www.iana.org/assignments/media-types/image/vnd.dwg> ;
  rdfs:seeAlso <https://www.opendesign.com/files/guestdownloads/OpenDesign_Specification_for_.dwg_files.pdf> ;
  rdfs:seeAlso wd:Q1053358 ;
  rdfs:subPropertyOf omg:hasSimpleGeometryDescription ;
.
fog:asDwg_v2010
  rdf:type owl:DatatypeProperty ;
  rdf:type owl:FunctionalProperty ;
  dbp:extension ".dwg" ;
  rdfs:comment "The datatype relation pointing to a geometry description following the proprietary DWG v2010 format from Autodesk. It consists of a single .dwg file (binary)."@en ;
  rdfs:isDefinedBy fog: ;
  rdfs:label "as DWG 2010 format (.dwg)"@en ;
  rdfs:subPropertyOf fog:asDwg ;
.
fog:asDwg_v2013
  rdf:type owl:DatatypeProperty ;
  rdf:type owl:FunctionalProperty ;
  dbp:extension ".dwg" ;
  rdfs:comment "The datatype relation pointing to a geometry description following the proprietary DWG v2013 format from Autodesk. It consists of a single .dwg file (binary)."@en ;
  rdfs:isDefinedBy fog: ;
  rdfs:label "as DWG 2013 format (.dwg)"@en ;
  rdfs:subPropertyOf fog:asDwg ;
.
fog:asDwg_v2018
  rdf:type owl:DatatypeProperty ;
  rdf:type owl:FunctionalProperty ;
  dbp:extension ".dwg" ;
  rdfs:comment "The datatype relation pointing to a geometry description following the proprietary DWG v2018 format from Autodesk. It consists of a single .dwg file (binary)."@en ;
  rdfs:isDefinedBy fog: ;
  rdfs:label "as DWG 2018 format (.dwg)"@en ;
  rdfs:subPropertyOf fog:asDwg ;
.
fog:asE57
  rdf:type owl:DatatypeProperty ;
  rdf:type owl:FunctionalProperty ;
  rdfs:comment "The datatype relation pointing to a point cloud geometry description following the open E57 format developed by the ASTM Committee E57. The format consists of a single .e57 file (partially binary, partially text-based). It is strongly adviced to use the more specific subproperties (e.g. fog:asE57_v1.0)."@en ;
  rdfs:isDefinedBy fog: ;
  rdfs:label "as E57 format"@en ;
  rdfs:seeAlso <https://www.astm.org/Standards/E2807.htm> ;
  rdfs:seeAlso <https://www.ri.cmu.edu/publications/the-astm-e57-file-format-for-3d-imaging-data-exchange/> ;
  rdfs:seeAlso wd:Q33517407 ;
  rdfs:subPropertyOf omg:hasSimpleGeometryDescription ;
.
<https://w3id.org/fog#asE57_v1.0>
  rdf:type owl:DatatypeProperty ;
  rdf:type owl:FunctionalProperty ;
  dbp:extension ".e57" ;
  rdfs:comment "The datatype relation pointing to a point cloud geometry description following the open E57 format developed by the ASTM Committee E57. The format consists of a single .e57 file (partially binary, partially text-based)."@en ;
  rdfs:isDefinedBy fog: ;
  rdfs:label "as E57 v1.0 format (.e57)"@en ;
  rdfs:seeAlso <https://www.astm.org/Standards/E2807.htm> ;
  rdfs:seeAlso <https://www.ri.cmu.edu/publications/the-astm-e57-file-format-for-3d-imaging-data-exchange/> ;
  rdfs:subPropertyOf fog:asE57 ;
.
fog:asGeojson
  rdf:type owl:DatatypeProperty ;
  rdf:type owl:FunctionalProperty ;
  rdfs:comment "The datatype relation pointing to a geometry description following the open GeoJSON format. The format consists of a single .json file (text-based). It is strongly adviced to use the more specific subproperties (e.g. fog:asGeojson_v2016). Note that the version proposed by the IETF GeoJSON Working Group (fog:asGeojson_v2016) is derived from the now obsolete 2008 version (fog:asGeojson_v2008)."@en ;
  rdfs:isDefinedBy fog: ;
  rdfs:label "as GeoJSON format"@en ;
  rdfs:seeAlso dbr:GeoJSON ;
  rdfs:seeAlso wd:Q5533904 ;
  rdfs:subPropertyOf omg:hasSimpleGeometryDescription ;
.
fog:asGeojson-ld
  rdf:type owl:FunctionalProperty ;
  rdf:type owl:ObjectProperty ;
  rdfs:comment "The object relation pointing to a GeoJSON-LD geometry description: a GeoJSON geometry description complemented with the corresponding JSON-LD context to make it RDF. It should be connected to the topnode of the geometry description. Note that this geometry description can only be used to depict single points, as the current JSON-LD specification v1.0 does not implement the deserialisation of nested lists to RDF"@en ;
  rdfs:isDefinedBy fog: ;
  rdfs:label "as GeoJSON-LD"@en ;
  rdfs:seeAlso <http://geojson.org/geojson-ld/> ;
  rdfs:subPropertyOf omg:hasComplexGeometryDescription ;
.
fog:asGeojson_v2008
  rdf:type owl:DatatypeProperty ;
  rdf:type owl:FunctionalProperty ;
  dbp:extension ".json" ;
  rdfs:comment "The datatype relation pointing to a geometry description following the open GeoJSON v2008 format. The format consists of a single .json file (text-based). Note that the version proposed by the IETF (fog:asGeojson_v2016) is derived from the now obsolete 2008 version (fog:asGeojson_v2008)."@en ;
  rdfs:isDefinedBy fog: ;
  rdfs:label "as GeoJSON format v2008 (.json)"@en ;
  rdfs:seeAlso <http://geojson.org/geojson-spec> ;
  rdfs:subPropertyOf fog:asGeojson ;
.
fog:asGeojson_v2016
  rdf:type owl:DatatypeProperty ;
  rdf:type owl:FunctionalProperty ;
  dbp:extension ".geojson" ;
  dbp:extension ".json" ;
  rdfs:comment "The datatype relation pointing to a geometry description following the open GeoJSON v2016 format developed by the IETF GeoJSON Working Group. The format consists of a single .json file (text-based). Note that the version proposed by the IETF (fog:asGeojson_v2016) is derived from the now obsolete 2008 version (fog:asGeojson_v2008)."@en ;
  rdfs:isDefinedBy fog: ;
  rdfs:label "as GeoJSON v2016 format (.json)"@en ;
  rdfs:seeAlso <https://tools.ietf.org/html/rfc7946> ;
  rdfs:seeAlso <https://www.iana.org/assignments/media-types/application/geo+json> ;
  rdfs:subPropertyOf fog:asGeojson ;
.
fog:asGeomOntology
  rdf:type owl:FunctionalProperty ;
  rdf:type owl:ObjectProperty ;
  rdfs:comment "The object relation pointing to a RDF-based geometry description following the GEOM ontology. It should be connected to the topnode of the geometry description."@en ;
  rdfs:isDefinedBy fog: ;
  rdfs:label "as GEOM ontology"@en ;
  rdfs:seeAlso <http://rdf.bg/geometry.ttl> ;
  rdfs:subPropertyOf omg:hasComplexGeometryDescription ;
.
fog:asGltf
  rdf:type owl:DatatypeProperty ;
  rdfs:comment "The datatype relation pointing to a geometry description following the open glTF format from the Khronos Group. The format consists of one (.gltf with embedded binary geometry/textures/shaders, or .glb) or multiple files (combination of binary and/or text-based files). It is strongly adviced to use the more specific subsubproperties (e.g. fog:asGltf_v2.0-gltf)."@en ;
  rdfs:isDefinedBy fog: ;
  rdfs:label "as glTF format"@en ;
  rdfs:subPropertyOf omg:hasSimpleGeometryDescription ;
.
<https://w3id.org/fog#asGltf_v1.0>
  rdf:type owl:DatatypeProperty ;
  rdfs:comment "The datatype relation pointing to a geometry description following the open glTF v1.0 format from the Khronos Group. The format consists of one (.gltf with embedded binary geometry/textures/shaders) or multiple files (combination of binary and/or text-based files). It is strongly adviced to use the more specific subproperties (e.g. fog:asGltf_v1.0-gltf)."@en ;
  rdfs:isDefinedBy fog: ;
  rdfs:label "as glTF v1.0 format"@en ;
  rdfs:seeAlso <https://github.com/KhronosGroup/glTF/tree/master/specification/1.0> ;
  rdfs:seeAlso wd:Q28135989 ;
  rdfs:subPropertyOf fog:asGltf ;
.
<https://w3id.org/fog#asGltf_v1.0-bin>
  rdf:type owl:DatatypeProperty ;
  rdf:type owl:FunctionalProperty ;
  dbp:extension ".bin" ;
  dcterms:requires "fog:asGltf_v1.0-gltf" ;
  rdfs:comment "The datatype relation pointing to a binary geometry file (.bin) following the open glTF v1.0 format from the Khronos Group. This file always has to be used together with the central .gltf JSON file (fog:asGltf_v1.0-gltf) referencing it."@en ;
  rdfs:isDefinedBy fog: ;
  rdfs:label "as glTF v1.0 geometry file (.bin)"@en ;
  rdfs:subPropertyOf <https://w3id.org/fog#asGltf_v1.0> ;
.
<https://w3id.org/fog#asGltf_v1.0-glsl>
  rdf:type owl:DatatypeProperty ;
  rdf:type owl:FunctionalProperty ;
  dbp:extension ".glsl" ;
  dcterms:requires "fog:asGltf_v1.0-gltf" ;
  rdfs:comment "The datatype relation pointing to a text-based shader file (.glsl) following the open glTF v1.0 format from the Khronos Group. This file always has to be used together with the central .gltf JSON file (fog:asGltf_v1.0-gltf) referencing it."@en ;
  rdfs:isDefinedBy fog: ;
  rdfs:label "as glTF v1.0 shader file (.glsl)"@en ;
  rdfs:subPropertyOf <https://w3id.org/fog#asGltf_v1.0> ;
.
<https://w3id.org/fog#asGltf_v1.0-gltf>
  rdf:type owl:DatatypeProperty ;
  rdf:type owl:FunctionalProperty ;
  dbp:extension ".gltf" ;
  rdfs:comment "The datatype relation pointing to a JSON file (.gltf) following the open glTF v1.0 format from the Khronos Group. This file can be used on its own if geometry, shaders and optional textures are embedded (text-based) inside the JSON. In most cases however, it references other files containing geometry (.bin), optional shaders (.glsl) and optional textures (.bmp/.gif/.jpeg/.png)."@en ;
  rdfs:isDefinedBy fog: ;
  rdfs:label "as glTF v1.0 JSON file (.gltf)"@en ;
  rdfs:seeAlso <https://www.iana.org/assignments/media-types/model/gltf+json> ;
  rdfs:subPropertyOf <https://w3id.org/fog#asGltf_v1.0> ;
.
<https://w3id.org/fog#asGltf_v1.0-texture>
  rdf:type owl:DatatypeProperty ;
  rdf:type owl:FunctionalProperty ;
  dbp:extension ".bmp" ;
  dbp:extension ".gif" ;
  dbp:extension ".jpeg" ;
  dbp:extension ".png" ;
  dcterms:requires "fog:asGltf_v1.0-gltf" ;
  rdfs:comment "The datatype relation pointing to a binary texture file (.bmp/..gif/.jpeg/.png). This file always has to be used together with the central .gltf JSON file (fog:asGltf_v1.0-gltf) referencing it."@en ;
  rdfs:isDefinedBy fog: ;
  rdfs:label "as glTF v1.0 texture file"@en ;
  rdfs:subPropertyOf <https://w3id.org/fog#asGltf_v1.0> ;
.
<https://w3id.org/fog#asGltf_v2.0>
  rdf:type owl:DatatypeProperty ;
  rdfs:comment "The datatype relation pointing to a geometry description following the open glTF v2.0 format from the Khronos Group. The format consists of one (.gltf with embedded binary geometry/textures/shaders, or .glb) or multiple files (combination of binary and/or text-based files). It is strongly adviced to use the more specific subproperties (e.g. fog:asGltf_v2.0-gltf)."@en ;
  rdfs:isDefinedBy fog: ;
  rdfs:label "as glTF v2.0 format"@en ;
  rdfs:seeAlso <https://github.com/KhronosGroup/glTF/tree/master/specification/2.0> ;
  rdfs:subPropertyOf fog:asGltf ;
.
<https://w3id.org/fog#asGltf_v2.0-bin>
  rdf:type owl:DatatypeProperty ;
  rdf:type owl:FunctionalProperty ;
  dbp:extension ".bin" ;
  dcterms:requires "fog:asGltf_v2.0-gltf" ;
  rdfs:comment "The datatype relation pointing to a binary geometry file (.bin) following the open glTF v2.0 format from the Khronos Group. This file always has to be used together with the central .gltf JSON file (fog:asGltf_v2.0-gltf) referencing it."@en ;
  rdfs:isDefinedBy fog: ;
  rdfs:label "as glTF v2.0 geometry file (.bin)"@en ;
  rdfs:seeAlso <https://www.iana.org/assignments/media-types/application/gltf-buffer> ;
  rdfs:subPropertyOf <https://w3id.org/fog#asGltf_v2.0> ;
.
<https://w3id.org/fog#asGltf_v2.0-glb>
  rdf:type owl:DatatypeProperty ;
  rdf:type owl:FunctionalProperty ;
  dbp:extension ".glb" ;
  rdfs:comment "The datatype relation pointing to a binary file (.glb) following the open glTF v2.0 format from the Khronos Group. This one file contains geometry and textures, and as a result can be used without other files."@en ;
  rdfs:isDefinedBy fog: ;
  rdfs:label "as glTF v2.0 binary file (.glb)"@en ;
  rdfs:seeAlso <https://www.iana.org/assignments/media-types/model/gltf-binary> ;
  rdfs:subPropertyOf <https://w3id.org/fog#asGltf_v2.0> ;
.
<https://w3id.org/fog#asGltf_v2.0-gltf>
  rdf:type owl:DatatypeProperty ;
  rdf:type owl:FunctionalProperty ;
  dbp:extension ".gltf" ;
  rdfs:comment "The datatype relation pointing to a JSON file (.gltf) following the open glTF v2.0 format from the Khronos Group. This file can be used on its own if geometry and optional textures are embedded (text-based) inside the JSON. In most cases however, it references other files containing geometry (.bin) and optional textures (.jpeg/.png)."@en ;
  rdfs:isDefinedBy fog: ;
  rdfs:label "as glTF v2.0 JSON file (.gltf)"@en ;
  rdfs:subPropertyOf <https://w3id.org/fog#asGltf_v2.0> ;
.
<https://w3id.org/fog#asGltf_v2.0-texture>
  rdf:type owl:DatatypeProperty ;
  rdf:type owl:FunctionalProperty ;
  dbp:extension ".jpeg" ;
  dbp:extension ".png" ;
  dcterms:requires "fog:asGltf_v2.0-gltf" ;
  rdfs:comment "The datatype relation pointing to a binary texture file (.jpeg/.png). This file always has to be used together with the central .gltf JSON file (fog:asGltf_v2.0-gltf) referencing it."@en ;
  rdfs:isDefinedBy fog: ;
  rdfs:label "as glTF v2.0 texture file"@en ;
  rdfs:subPropertyOf <https://w3id.org/fog#asGltf_v2.0> ;
.
fog:asGml
  rdf:type owl:DatatypeProperty ;
  rdf:type owl:FunctionalProperty ;
  rdfs:comment "The datatype relation pointing to a text-based geometry description following one of the open GML formats developed by OGC and ISO. The format consists of a single .gml file (text-based). It is strongly adviced to use the more specific subproperties (e.g. fog:asGml_v3.3.0). Note that this property is disjoint with geo:asGML because of the more strict domain and range restrictions in GeoSPARQL."@en ;
  rdfs:isDefinedBy fog: ;
  rdfs:label "as GML format"@en ;
  rdfs:seeAlso <http://schemas.opengis.net/gml/> ;
  rdfs:seeAlso <https://www.opengeospatial.org/standards/gml> ;
  rdfs:seeAlso wd:Q926165 ;
  rdfs:subPropertyOf omg:hasSimpleGeometryDescription ;
  owl:propertyDisjointWith geo:asGML ;
.
<https://w3id.org/fog#asGml_v3.1.1>
  rdf:type owl:DatatypeProperty ;
  rdf:type owl:FunctionalProperty ;
  dbp:extension ".gml" ;
  rdfs:comment "The datatype relation pointing to a text-based GML file (.gml) following the open GML v3.1.1 format developed by OGC and ISO. Note that this and older versions are considered depreciated. Note that this property is disjoint (via its superproperty fog:asGml) with geo:asGML because of the more strict domain and range restrictions in GeoSPARQL."@en ;
  rdfs:isDefinedBy fog: ;
  rdfs:label "as GML v3.1.1 format (.gml)"@en ;
  rdfs:seeAlso <http://portal.opengeospatial.org/files/?artifact_id=4700> ;
  rdfs:seeAlso <http://schemas.opengis.net/gml/3.1.1/> ;
  rdfs:subPropertyOf fog:asGml ;
.
<https://w3id.org/fog#asGml_v3.2.1>
  rdf:type owl:DatatypeProperty ;
  rdf:type owl:FunctionalProperty ;
  dbp:extension ".gml" ;
  rdfs:comment "The datatype relation pointing to a text-based GML file (.gml) following the open GML v3.2.1 format developed by OGC and ISO. Note that this property is disjoint (via its superproperty fog:asGml) with geo:asGML because of the more strict domain and range restrictions in GeoSPARQL."@en ;
  rdfs:isDefinedBy fog: ;
  rdfs:label "as GML v3.2.1 format (.gml)"@en ;
  rdfs:seeAlso <http://portal.opengeospatial.org/files/?artifact_id=20509> ;
  rdfs:seeAlso <http://schemas.opengis.net/gml/3.2.1/> ;
  rdfs:subPropertyOf fog:asGml ;
.
<https://w3id.org/fog#asGml_v3.2.2>
  rdf:type owl:DatatypeProperty ;
  rdf:type owl:FunctionalProperty ;
  dbp:extension ".gml" ;
  rdfs:comment "The datatype relation pointing to a text-based GML file (.gml) following the open GML v3.2.2 format developed by OGC and ISO. Note that this property is disjoint (via its superproperty fog:asGml) with geo:asGML because of the more strict domain and range restrictions in GeoSPARQL."@en ;
  rdfs:isDefinedBy fog: ;
  rdfs:label "as GML v3.2.2 format (.gml)"@en ;
  rdfs:seeAlso <https://portal.opengeospatial.org/files/?artifact_id=74183&version=2> ;
  rdfs:subPropertyOf fog:asGml ;
.
<https://w3id.org/fog#asGml_v3.3.0>
  rdf:type owl:DatatypeProperty ;
  rdf:type owl:FunctionalProperty ;
  dbp:extension ".gml" ;
  rdfs:comment "The datatype relation pointing to a text-based GML file (.gml) following the open GML v3.3.0 format developed by OGC and ISO. This format is an extension of the GML v3.2 format. Note that this property is disjoint (via its superproperty fog:asGml) with geo:asGML because of the more strict domain and range restrictions in GeoSPARQL."@en ;
  rdfs:isDefinedBy fog: ;
  rdfs:label "as GML v3.3.0 format (.gml)"@en ;
  rdfs:seeAlso <http://schemas.opengis.net/gml/3.3/> ;
  rdfs:seeAlso <https://portal.opengeospatial.org/files/?artifact_id=46568> ;
  rdfs:subPropertyOf fog:asGml ;
.
fog:asIfc
  rdf:type owl:DatatypeProperty ;
  rdf:type owl:FunctionalProperty ;
  rdfs:comment "The datatype relation pointing to a text-based geometry description following the open IFC format as documented by buildingSMART and in its ISO 16739 standard. The format consists of a single .ifc or .ifcxml file (text-based). It is strongly adviced to use the more specific subproperties (e.g. fog:asIfc_v2x4-icfxml)."@en ;
  rdfs:isDefinedBy fog: ;
  rdfs:label "as IFC format"@en ;
  rdfs:seeAlso dbr:Industry_Foundation_Classes ;
  rdfs:seeAlso <https://www.iso.org/standard/70303.html> ;
  rdfs:seeAlso wd:Q979630 ;
  rdfs:subPropertyOf omg:hasSimpleGeometryDescription ;
.
fog:asIfc_v2x3
  rdf:type owl:DatatypeProperty ;
  rdf:type owl:FunctionalProperty ;
  rdfs:comment "The datatype relation pointing to a text-based geometry description following the open IFC format v2x3 as documented by buildingSMART and in its ISO 16739 standard"@en ;
  rdfs:isDefinedBy fog: ;
  rdfs:label "as IFC v2x3"@en ;
  rdfs:seeAlso <http://www.buildingsmart-tech.org/specifications/ifc-releases/ifc2x3-release> ;
  rdfs:subPropertyOf fog:asIfc ;
.
fog:asIfc_v2x3-ifc
  rdf:type owl:DatatypeProperty ;
  rdf:type owl:FunctionalProperty ;
  dbp:extension ".ifc" ;
  rdfs:comment "The datatype relation pointing to a text-based geometry description following the open IFC format v2x3 as documented by buildingSMART and in its ISO 16739 standard. The IFC file is serialised in the STEP Physical File Format (SPFF)."@en ;
  rdfs:isDefinedBy fog: ;
  rdfs:label "as IFC v2x3 file (.ifc)"@en ;
  rdfs:subPropertyOf fog:asIfc_v2x3 ;
.
fog:asIfc_v2x3-ifcxml
  rdf:type owl:DatatypeProperty ;
  rdf:type owl:FunctionalProperty ;
  dbp:extension ".ifcxml" ;
  rdfs:comment "The datatype relation pointing to a text-based geometry description following the open IFC format v2x3 as documented by buildingSMART and in its ISO 16739 standard. The IFC file is serialised in the XML format."@en ;
  rdfs:isDefinedBy fog: ;
  rdfs:label "as IFC v2x3 file (.ifcxml)"@en ;
  rdfs:subPropertyOf fog:asIfc_v2x3 ;
.
fog:asIfc_v2x3tc1
  rdf:type owl:DatatypeProperty ;
  rdf:type owl:FunctionalProperty ;
  rdfs:comment "The datatype relation pointing to a text-based geometry description following the open IFC format v2x3 TC1 as documented by buildingSMART and in its ISO 16739 standard"@en ;
  rdfs:isDefinedBy fog: ;
  rdfs:label "as IFC v2x3 TC1"@en ;
  rdfs:seeAlso <http://www.buildingsmart-tech.org/specifications/ifc-releases/ifc2x3-tc1-release> ;
  rdfs:subPropertyOf fog:asIfc ;
.
fog:asIfc_v2x3tc1-ifc
  rdf:type owl:DatatypeProperty ;
  rdf:type owl:FunctionalProperty ;
  dbp:extension ".ifc" ;
  rdfs:comment "The datatype relation pointing to a text-based geometry description following the open IFC format v2x3 TC1 as documented by buildingSMART and in its ISO 16739 standard. The IFC file is serialised in the STEP Physical File Format (SPFF)."@en ;
  rdfs:isDefinedBy fog: ;
  rdfs:label "as IFC v2x3 TC1 file (.ifc)"@en ;
  rdfs:subPropertyOf fog:asIfc_v2x3tc1 ;
.
fog:asIfc_v2x3tc1-ifcxml
  rdf:type owl:DatatypeProperty ;
  rdf:type owl:FunctionalProperty ;
  dbp:extension ".ifcxml" ;
  rdfs:comment "The datatype relation pointing to a text-based geometry description following the open IFC format v2x3 TC1 as documented by buildingSMART and in its ISO 16739 standard. The IFC file is serialised in the XML format."@en ;
  rdfs:isDefinedBy fog: ;
  rdfs:label "as IFC v2x3 TC1 file (.ifcxml)"@en ;
  rdfs:subPropertyOf fog:asIfc_v2x3tc1 ;
.
fog:asIfc_v2x4
  rdf:type owl:DatatypeProperty ;
  rdf:type owl:FunctionalProperty ;
  rdfs:comment "The datatype relation pointing to a text-based geometry description following the open IFC format v2x4 as documented by buildingSMART and in its ISO 16739 standard"@en ;
  rdfs:isDefinedBy fog: ;
  rdfs:label "as IFC v2x4"@en ;
  rdfs:seeAlso <http://www.buildingsmart-tech.org/specifications/ifc-releases/ifc4-release> ;
  rdfs:subPropertyOf fog:asIfc ;
.
fog:asIfc_v2x4-ifc
  rdf:type owl:DatatypeProperty ;
  rdf:type owl:FunctionalProperty ;
  dbp:extension ".ifc" ;
  rdfs:comment "The datatype relation pointing to a text-based geometry description following the open IFC format v2x4 as documented by buildingSMART and in its ISO 16739 standard. The IFC file is serialised in the STEP Physical File Format (SPFF)."@en ;
  rdfs:isDefinedBy fog: ;
  rdfs:label "as IFC v2x4 file (.ifc)"@en ;
  rdfs:subPropertyOf fog:asIfc_v2x4 ;
.
fog:asIfc_v2x4-ifcxml
  rdf:type owl:DatatypeProperty ;
  rdf:type owl:FunctionalProperty ;
  dbp:extension ".ifcxml" ;
  rdfs:comment "The datatype relation pointing to a text-based geometry description following the open IFC format v2x4 as documented by buildingSMART and in its ISO 16739 standard. The IFC file is serialised in the XML format."@en ;
  rdfs:isDefinedBy fog: ;
  rdfs:label "as IFC v2x4 file (.ifcxml)"@en ;
  rdfs:subPropertyOf fog:asIfc_v2x4 ;
.
fog:asIfc_v2x4add1
  rdf:type owl:DatatypeProperty ;
  rdf:type owl:FunctionalProperty ;
  rdfs:comment "The datatype relation pointing to a text-based geometry description following the open IFC format v2x4 Add1 as documented by buildingSMART and in its ISO 16739 standard"@en ;
  rdfs:isDefinedBy fog: ;
  rdfs:label "as IFC v2x4 Add1"@en ;
  rdfs:seeAlso <http://www.buildingsmart-tech.org/specifications/ifc-releases/ifc4-add1-release> ;
  rdfs:subPropertyOf fog:asIfc ;
.
fog:asIfc_v2x4add1-ifc
  rdf:type owl:DatatypeProperty ;
  rdf:type owl:FunctionalProperty ;
  dbp:extension ".ifc" ;
  rdfs:comment "The datatype relation pointing to a text-based geometry description following the open IFC format v2x4 Add1 as documented by buildingSMART and in its ISO 16739 standard. The IFC file is serialised in the STEP Physical File Format (SPFF)."@en ;
  rdfs:isDefinedBy fog: ;
  rdfs:label "as IFC v2x4 Add1 file (.ifc)"@en ;
  rdfs:subPropertyOf fog:asIfc_v2x4add1 ;
.
fog:asIfc_v2x4add1-ifcxml
  rdf:type owl:DatatypeProperty ;
  rdf:type owl:FunctionalProperty ;
  dbp:extension ".ifcxml" ;
  rdfs:comment "The datatype relation pointing to a text-based geometry description following the open IFC format v2x4 Add1 as documented by buildingSMART and in its ISO 16739 standard. The IFC file is serialised in the XML format."@en ;
  rdfs:isDefinedBy fog: ;
  rdfs:label "as IFC v2x4 Add1 file (.ifcxml)"@en ;
  rdfs:subPropertyOf fog:asIfc_v2x4add1 ;
.
fog:asIfc_v2x4add2
  rdf:type owl:DatatypeProperty ;
  rdf:type owl:FunctionalProperty ;
  rdfs:comment "The datatype relation pointing to a text-based geometry description following the open IFC format v2x4 Add2 as documented by buildingSMART and in its ISO 16739 standard"@en ;
  rdfs:isDefinedBy fog: ;
  rdfs:label "as IFC v2x4 Add2"@en ;
  rdfs:seeAlso <http://www.buildingsmart-tech.org/specifications/ifc-releases/ifc4-add2> ;
  rdfs:subPropertyOf fog:asIfc ;
.
fog:asIfc_v2x4add2-ifc
  rdf:type owl:DatatypeProperty ;
  rdf:type owl:FunctionalProperty ;
  dbp:extension ".ifc" ;
  rdfs:comment "The datatype relation pointing to a text-based geometry description following the open IFC format v2x4 Add2 as documented by buildingSMART and in its ISO 16739 standard. The IFC file is serialised in the STEP Physical File Format (SPFF)."@en ;
  rdfs:isDefinedBy fog: ;
  rdfs:label "as IFC v2x4 Add2 file (.ifc)"@en ;
  rdfs:subPropertyOf fog:asIfc_v2x4add2 ;
.
fog:asIfc_v2x4add2-ifcxml
  rdf:type owl:DatatypeProperty ;
  rdf:type owl:FunctionalProperty ;
  dbp:extension ".ifcxml" ;
  rdfs:comment "The datatype relation pointing to a text-based geometry description following the open IFC format v2x4 Add2 as documented by buildingSMART and in its ISO 16739 standard. The IFC file is serialised in the XML format."@en ;
  rdfs:isDefinedBy fog: ;
  rdfs:label "as IFC v2x4 Add 2 file (.ifcxml)"@en ;
  rdfs:subPropertyOf fog:asIfc_v2x4add2 ;
.
fog:asIfcowl
  rdf:type owl:FunctionalProperty ;
  rdf:type owl:ObjectProperty ;
  rdfs:comment "The object relation pointing to a RDF-based geometry description following the IfcOWL ontology."@en ;
  rdfs:isDefinedBy fog: ;
  rdfs:label "as ifcOWL ontology"@en ;
  rdfs:seeAlso <http://standards.buildingsmart.org/IFC/DEV/> ;
  rdfs:subPropertyOf omg:hasComplexGeometryDescription ;
.
fog:asIfcowl_v2x3final
  rdf:type owl:FunctionalProperty ;
  rdf:type owl:ObjectProperty ;
  rdfs:comment "The object relation pointing to a RDF-based geometry description following the IfcOWL v2x3 Final ontology."@en ;
  rdfs:isDefinedBy fog: ;
  rdfs:label "as ifcOWL v2x3 Final ontology"@en ;
  rdfs:seeAlso <https://standards.buildingsmart.org/IFC/DEV/IFC2x3/FINAL/OWL> ;
  rdfs:subPropertyOf fog:asIfcowl ;
.
fog:asIfcowl_v2x3tc1
  rdf:type owl:FunctionalProperty ;
  rdf:type owl:ObjectProperty ;
  rdfs:comment "The object relation pointing to a RDF-based geometry description following the IfcOWL v2x3 TC1 ontology."@en ;
  rdfs:isDefinedBy fog: ;
  rdfs:label "as ifcOWL v2x3 TC1 ontology"@en ;
  rdfs:seeAlso <https://standards.buildingsmart.org/IFC/DEV/IFC2x3/TC1/OWL> ;
  rdfs:subPropertyOf fog:asIfcowl ;
.
fog:asIfcowl_v2x4add1
  rdf:type owl:FunctionalProperty ;
  rdf:type owl:ObjectProperty ;
  rdfs:comment "The object relation pointing to a RDF-based geometry description following the IfcOWL v2x4 Add1 ontology."@en ;
  rdfs:isDefinedBy fog: ;
  rdfs:label "as ifcOWL v2x4 Add1 ontology"@en ;
  rdfs:seeAlso <https://standards.buildingsmart.org/IFC/DEV/IFC4/ADD1/OWL> ;
  rdfs:subPropertyOf fog:asIfcowl ;
.
fog:asIfcowl_v2x4add2
  rdf:type owl:FunctionalProperty ;
  rdf:type owl:ObjectProperty ;
  rdfs:comment "The object relation pointing to a RDF-based geometry description following the IfcOWL v2x4 Add2 ontology."@en ;
  rdfs:isDefinedBy fog: ;
  rdfs:label "as ifcOWL v2x4 Add2 ontology"@en ;
  rdfs:seeAlso <https://standards.buildingsmart.org/IFC/DEV/IFC4/ADD2/OWL> ;
  rdfs:subPropertyOf fog:asIfcowl ;
.
fog:asIfcowl_v2x4final
  rdf:type owl:FunctionalProperty ;
  rdf:type owl:ObjectProperty ;
  rdfs:comment "The object relation pointing to a RDF-based geometry description following the IfcOWL v2x4 Final ontology."@en ;
  rdfs:isDefinedBy fog: ;
  rdfs:label "as ifcOWL v2x4 Final ontology"@en ;
  rdfs:seeAlso <https://standards.buildingsmart.org/IFC/DEV/IFC4/FINAL/OWL> ;
  rdfs:subPropertyOf fog:asIfcowl ;
.
fog:asIges
  rdf:type owl:DatatypeProperty ;
  rdf:type owl:FunctionalProperty ;
  dbp:extension ".iges" ;
  dbp:extension ".igs" ;
  rdfs:comment "The datatype relation pointing to a geometry description following the IGES format as documented in its ANSI standard. The format consists of a single .iges/.igs file (text-based). It is strongly adviced to use the more specific subproperties (e.g. fog:asIges_v5.3)."@en ;
  rdfs:isDefinedBy fog: ;
  rdfs:label "as IGES format"@en ;
  rdfs:seeAlso dbr:IGES ;
  rdfs:seeAlso <https://www.iana.org/assignments/media-types/model/iges> ;
  rdfs:seeAlso wd:Q616714 ;
  rdfs:subPropertyOf omg:hasSimpleGeometryDescription ;
.
<https://w3id.org/fog#asIges_v5.3>
  rdf:type owl:DatatypeProperty ;
  rdf:type owl:FunctionalProperty ;
  dbp:extension ".iges" ;
  dbp:extension ".igs" ;
  rdfs:comment "The datatype relation pointing to a geometry description following the IGES format v5.6 as documented in its ANSI standard."@en ;
  rdfs:isDefinedBy fog: ;
  rdfs:label "as IGES v5.3 (.igs)"@en ;
  rdfs:subPropertyOf fog:asIges ;
.
fog:asLas
  rdf:type owl:DatatypeProperty ;
  rdf:type owl:FunctionalProperty ;
  rdfs:comment "The datatype relation pointing to a binary encoded point cloud following the open LAS format which was developed by the ASPRS. The format consists of a single .las or .laz file (binary). It is strongly adviced to use the more specific subproperties (e.g. fog:asLas_v1.4-las)."@en ;
  rdfs:isDefinedBy fog: ;
  rdfs:label "as LAS point cloud format"@en ;
  rdfs:seeAlso <https://github.com/ASPRSorg/LAS> ;
  rdfs:seeAlso wd:Q27441566 ;
  rdfs:subPropertyOf omg:hasSimpleGeometryDescription ;
.
<https://w3id.org/fog#asLas_v1.4>
  rdf:type owl:DatatypeProperty ;
  rdf:type owl:FunctionalProperty ;
  rdfs:comment "The datatype relation pointing to a binary encoded point cloud following the v1.4 of the open LAS format which was developed by the ASPRS. The format consists of a single .las or .laz file (binary). It is strongly adviced to use the more specific subproperties (e.g. fog:asLas_v1.4-las)."@en ;
  rdfs:isDefinedBy fog: ;
  rdfs:label "as LAS v1.4 point cloud format"@en ;
  rdfs:seeAlso <http://www.asprs.org/wp-content/uploads/2019/03/LAS_1_4_r14.pdf> ;
  rdfs:seeAlso wd:Q33515758 ;
  rdfs:subPropertyOf fog:asLas ;
.
<https://w3id.org/fog#asLas_v1.4-las>
  rdf:type owl:DatatypeProperty ;
  rdf:type owl:FunctionalProperty ;
  dbp:extension ".las" ;
  rdfs:comment "The datatype relation pointing to an uncompressed binary encoded point cloud (.las) following the v1.4 of the open LAS format which was developed by the ASPRS."@en ;
  rdfs:isDefinedBy fog: ;
  rdfs:label "as uncompressed LAS v1.4 point cloud format (.las)"@en ;
  rdfs:subPropertyOf <https://w3id.org/fog#asLas_v1.4> ;
.
<https://w3id.org/fog#asLas_v1.4-laz>
  rdf:type owl:DatatypeProperty ;
  rdf:type owl:FunctionalProperty ;
  dbp:extension ".laz" ;
  rdfs:comment "The datatype relation pointing to a compressed binary encoded point cloud (.laz) following the v1.4 of the open LAS format which was developed by the ASPRS."@en ;
  rdfs:isDefinedBy fog: ;
  rdfs:label "as compressed LAS v1.4 point cloud format (.laz)"@en ;
  rdfs:subPropertyOf <https://w3id.org/fog#asLas_v1.4> ;
.
fog:asNexus
  rdf:type owl:DatatypeProperty ;
  rdf:type owl:FunctionalProperty ;
  rdfs:comment "The datatype relation pointing to a geometry description following the Nexus format for multiresoltion meshes and point clouds (ISTI - Italian National Research Council - Visual Computing Lab). The format consists of a single .nxs or .nxz file (binary). It is strongly adviced to use the more specific subproperties (e.g. fog:asNexus_v4.2-nxs)"@en ;
  rdfs:isDefinedBy fog: ;
  rdfs:label "as Nexus format"@en ;
  rdfs:seeAlso <http://vcg.isti.cnr.it/nexus/> ;
  rdfs:seeAlso <https://github.com/cnr-isti-vclab/nexus> ;
  rdfs:subPropertyOf omg:hasSimpleGeometryDescription ;
.
<https://w3id.org/fog#asNexus_v4.2>
  rdf:type owl:DatatypeProperty ;
  rdf:type owl:FunctionalProperty ;
  rdfs:comment "The datatype relation pointing to a geometry description following the Nexus v4.2 format for multiresoltion meshes and point clouds (ISTI - Italian National Research Council - Visual Computing Lab). The format consists of a single .nxs or .nxz file (binary). It is strongly adviced to use the more specific subproperties (e.g. fog:asNexus_v4.2-nxs)"@en ;
  rdfs:isDefinedBy fog: ;
  rdfs:label "as Nexus v4.2 format"@en ;
  rdfs:seeAlso <http://vcg.isti.cnr.it/nexus/> ;
  rdfs:seeAlso <https://github.com/cnr-isti-vclab/nexus> ;
  rdfs:subPropertyOf fog:asNexus ;
.
<https://w3id.org/fog#asNexus_v4.2-nxs>
  rdf:type owl:DatatypeProperty ;
  rdf:type owl:FunctionalProperty ;
  dbp:extension ".nxs" ;
  rdfs:comment "The datatype relation pointing to a geometry description following the uncompressed Nexus v4.2 format (.nxs) for multiresoltion meshes and point clouds (ISTI - Italian National Research Council - Visual Computing Lab)."@en ;
  rdfs:isDefinedBy fog: ;
  rdfs:label "as uncompressed Nexus v4.2 format (.nxs)"@en ;
  rdfs:subPropertyOf <https://w3id.org/fog#asNexus_v4.2> ;
.
<https://w3id.org/fog#asNexus_v4.2-nxz>
  rdf:type owl:DatatypeProperty ;
  rdf:type owl:FunctionalProperty ;
  dbp:extension ".nxz" ;
  rdfs:comment "The datatype relation pointing to a geometry description following the compressed Nexus v4.2 format (.nxz) for multiresoltion meshes and point clouds (ISTI - Italian National Research Council - Visual Computing Lab)."@en ;
  rdfs:isDefinedBy fog: ;
  rdfs:label "as compressed Nexus v4.2 format (.nxz)"@en ;
  rdfs:subPropertyOf <https://w3id.org/fog#asNexus_v4.2> ;
.
fog:asObj
  rdf:type owl:DatatypeProperty ;
  rdfs:comment "The datatype relation pointing to a text-based geometry description following the OBJ format developed by Wavefront Technologies. The format consists of a single .obj file and an optional material file (.mtl). It is strongly adviced to use the more specific subsubproperties (e.g. fog:asObj_v3.0-obj)."@en ;
  rdfs:isDefinedBy fog: ;
  rdfs:label "as OBJ format"@en ;
  rdfs:seeAlso <http://paulbourke.net/dataformats/obj/> ;
  rdfs:seeAlso wd:Q2119595 ;
  rdfs:subPropertyOf omg:hasSimpleGeometryDescription ;
.
<https://w3id.org/fog#asObj_v3.0>
  rdf:type owl:DatatypeProperty ;
  rdfs:comment "The datatype relation pointing to a text-based geometry description following the OBJ v3.0 format developed by Wavefront Technologies. The format consists of a single .obj file and an optional material file (.mtl). It is strongly adviced to use the more specific subproperties (e.g. fog:asObj_v3.0-obj)."@en ;
  rdfs:isDefinedBy fog: ;
  rdfs:label "as OBJ v3.0 format"@en ;
  rdfs:subPropertyOf fog:asObj ;
.
<https://w3id.org/fog#asObj_v3.0-mtl>
  rdf:type owl:DatatypeProperty ;
  rdf:type owl:FunctionalProperty ;
  dbp:extension ".mtl" ;
  dcterms:requires "fog:asObj_v3.0-obj" ;
  rdfs:comment "The datatype relation pointing to a text-based MTL file (.mtl) following the OBJ format developed by Wavefront Technologies. This file has to be used together with the main .obj file that references it."@en ;
  rdfs:isDefinedBy fog: ;
  rdfs:label "as OBJ v3.0 material file (.mtl)"@en ;
  rdfs:seeAlso wd:Q20965861 ;
  rdfs:seeAlso wd:Q38343645 ;
  rdfs:subPropertyOf <https://w3id.org/fog#asObj_v3.0> ;
.
<https://w3id.org/fog#asObj_v3.0-obj>
  rdf:type owl:DatatypeProperty ;
  rdf:type owl:FunctionalProperty ;
  dbp:extension ".obj" ;
  rdfs:comment "The datatype relation pointing to a text-based OBJ file (.obj) following the OBJ format developed by Wavefront Technologies. This file can be used together with an optional material file (.mtl)."@en ;
  rdfs:isDefinedBy fog: ;
  rdfs:label "as OBJ v3.0 file (.obj)"@en ;
  rdfs:subPropertyOf <https://w3id.org/fog#asObj_v3.0> ;
.
<https://w3id.org/fog#asObj_v3.0-texture>
  rdf:type owl:DatatypeProperty ;
  rdf:type owl:FunctionalProperty ;
  rdfs:comment "The datatype relation pointing to a binary texture file that is referenced in the .mtl file of the OBJ format."@en ;
  rdfs:isDefinedBy fog: ;
  rdfs:label "as OBJ texture"@en ;
  rdfs:subPropertyOf <https://w3id.org/fog#asObj_v3.0> ;
.
fog:asOntobrepOntology
  rdf:type owl:FunctionalProperty ;
  rdf:type owl:ObjectProperty ;
  rdfs:comment "The object relation pointing to a RDF-based geometry description following the OntoBREP ontology. It should be connected to the topnode of the geometry description."@en ;
  rdfs:isDefinedBy fog: ;
  rdfs:label "as OntoBREP ontology"@en ;
  rdfs:seeAlso <https://github.com/OntoBREP/ontobrep> ;
  rdfs:subPropertyOf omg:hasComplexGeometryDescription ;
.
fog:asOntostepOntology
  rdf:type owl:FunctionalProperty ;
  rdf:type owl:ObjectProperty ;
  rdfs:comment "The object relation pointing to a RDF-based geometry description following the OntoSTEP ontology. It should be connected to the topnode of the geometry description."@en ;
  rdfs:isDefinedBy fog: ;
  rdfs:label "as OntoSTEP ontology"@en ;
  rdfs:seeAlso <https://www.nist.gov/publications/ontostep-owl-dl-ontology-step?pub_id=901544> ;
  rdfs:subPropertyOf omg:hasComplexGeometryDescription ;
.
fog:asPcd
  rdf:type owl:DatatypeProperty ;
  rdf:type owl:FunctionalProperty ;
  rdfs:comment "The datatype relation pointing to a binary encoded point cloud following the open PCD format which was developed as part of the open source project PCL (point cloud library). The format consists of a single .pcd file (binary or text-based). It is strongly adviced to use the more specific subproperties (e.g. fog:asPcd_v0.7)."@en ;
  rdfs:isDefinedBy fog: ;
  rdfs:label "as PCD point cloud format"@en ;
  rdfs:seeAlso <http://pointclouds.org/documentation/tutorials/pcd_file_format.php> ;
  rdfs:subPropertyOf omg:hasSimpleGeometryDescription ;
.
<https://w3id.org/fog#asPcd_v0.7>
  rdf:type owl:DatatypeProperty ;
  rdf:type owl:FunctionalProperty ;
  dbp:extension ".pcd" ;
  rdfs:comment "The datatype relation pointing to a binary or text-based point cloud following the open PCD v0.7 (sometimes referred to as PCD_v7) format which was developed as part of the open source project PCL (point cloud library)."@en ;
  rdfs:isDefinedBy fog: ;
  rdfs:label "as PCD v0.7 point cloud format (.pcd)"@en ;
  rdfs:subPropertyOf fog:asPcd ;
.
<https://w3id.org/fog#asPcd_v0.7-ascii>
  rdf:type owl:DatatypeProperty ;
  rdf:type owl:FunctionalProperty ;
  dbp:extension ".pcd" ;
  rdfs:comment "The datatype relation pointing to a text-based point cloud following the open PCD v0.7 (sometimes referred to as PCD_v7) format which was developed as part of the open source project PCL (point cloud library)."@en ;
  rdfs:isDefinedBy fog: ;
  rdfs:label "as PCD v0.7 ASCII point cloud format (.pcd)"@en ;
  rdfs:subPropertyOf <https://w3id.org/fog#asPcd_v0.7> ;
.
<https://w3id.org/fog#asPcd_v0.7-binary>
  rdf:type owl:DatatypeProperty ;
  rdf:type owl:FunctionalProperty ;
  dbp:extension ".pcd" ;
  rdfs:comment "The datatype relation pointing to a binary point cloud following the open PCD v0.7 (sometimes referred to as PCD_v7) format which was developed as part of the open source project PCL (point cloud library)."@en ;
  rdfs:isDefinedBy fog: ;
  rdfs:label "as PCD v0.7 binary point cloud format (.pcd)"@en ;
  rdfs:subPropertyOf <https://w3id.org/fog#asPcd_v0.7> ;
.
fog:asPly
  rdf:type owl:DatatypeProperty ;
  rdf:type owl:FunctionalProperty ;
  dbp:extension ".ply" ;
  rdfs:comment "The datatype relation pointing to a geometry description following the PLY format which was developed by Greg Turk (Stanford University). The format consists of a single .ply file which is either text-based or binary. It is strongly adviced to use the more specific subsubproperties (e.g. fog:asPly_v1.0-ascii)."@en ;
  rdfs:isDefinedBy fog: ;
  rdfs:label "as PLY format" ;
  rdfs:seeAlso <http://dbpedia.org/resource/PLY_(file_format)> ;
  rdfs:seeAlso <http://paulbourke.net/dataformats/ply/> ;
  rdfs:seeAlso wd:Q3077345 ;
  rdfs:subPropertyOf omg:hasSimpleGeometryDescription ;
.
<https://w3id.org/fog#asPly_v1.0>
  rdf:type owl:DatatypeProperty ;
  rdf:type owl:FunctionalProperty ;
  rdfs:comment "The datatype relation pointing to a geometry description following the PLY v1.0 format which was developed by Greg Turk (Stanford University). The format consists of a single .ply file which is either text-based or binary. It is strongly adviced to use the more specific subproperties (e.g. fog:asPly_v1.0-ascii)."@en ;
  rdfs:isDefinedBy fog: ;
  rdfs:label "as PLY v1.0 format"@en ;
  rdfs:subPropertyOf fog:asPly ;
.
<https://w3id.org/fog#asPly_v1.0-ascii>
  rdf:type owl:DatatypeProperty ;
  rdf:type owl:FunctionalProperty ;
  dbp:extension ".ply" ;
  rdfs:comment "The datatype relation pointing to a geometry file following the PLY v1.0 format which was developed by Greg Turk (Stanford University). The single .ply file is text-based."@en ;
  rdfs:isDefinedBy fog: ;
  rdfs:label "as PLY v1.0 ASCII format (.ply)"@en ;
  rdfs:subPropertyOf <https://w3id.org/fog#asPly_v1.0> ;
.
<https://w3id.org/fog#asPly_v1.0-binaryBE>
  rdf:type owl:DatatypeProperty ;
  rdf:type owl:FunctionalProperty ;
  dbp:extension ".ply" ;
  rdfs:comment "The datatype relation pointing to a geometry file following the PLY v1.0 format which was developed by Greg Turk (Stanford University). The single .ply file is binary with big endian. Note that there is also a sibling property for a binary PLY with little endian."@en ;
  rdfs:isDefinedBy fog: ;
  rdfs:label "as PLY v1.0 binary (big endian) format (.ply)"@en ;
  rdfs:subPropertyOf <https://w3id.org/fog#asPly_v1.0> ;
.
<https://w3id.org/fog#asPly_v1.0-binaryLE>
  rdf:type owl:DatatypeProperty ;
  rdf:type owl:FunctionalProperty ;
  dbp:extension ".ply" ;
  rdfs:comment "The datatype relation pointing to a geometry file following the PLY v1.0 format which was developed by Greg Turk (Stanford University). The single .ply file is binary with little endian. Note that there is also a sibling property for a binary PLY with big endian."@en ;
  rdfs:isDefinedBy fog: ;
  rdfs:label "as PLY v1.0 binary (little endian) format (.ply)"@en ;
  rdfs:subPropertyOf <https://w3id.org/fog#asPly_v1.0> ;
.
fog:asRevit
  rdf:type owl:DatatypeProperty ;
  rdf:type owl:FunctionalProperty ;
  dbp:extension ".rvt" ;
  rdfs:comment "The datatype relation pointing to a geometry description following the proprietary Revit format (Autodesk). The format consists of a single .rvt file (binary). It is strongly adviced to use the more specific subproperties (e.g. fog:asRevit_v2020)"@en ;
  rdfs:isDefinedBy fog: ;
  rdfs:label "as Revit format"@en ;
  rdfs:seeAlso wd:Q49620191 ;
  rdfs:subPropertyOf omg:hasSimpleGeometryDescription ;
.
fog:asRevit_v2017
  rdf:type owl:DatatypeProperty ;
  rdf:type owl:FunctionalProperty ;
  dbp:extension ".rvt" ;
  rdfs:comment "The datatype relation pointing to a geometry description following the proprietary Revit v2017 format (Autodesk). The format consists of a single .rvt file (binary)."@en ;
  rdfs:isDefinedBy fog: ;
  rdfs:label "as Revit format v2017 (.rvt)"@en ;
  rdfs:subPropertyOf fog:asRevit ;
.
fog:asRevit_v2018
  rdf:type owl:DatatypeProperty ;
  rdf:type owl:FunctionalProperty ;
  dbp:extension ".rvt" ;
  rdfs:comment "The datatype relation pointing to a geometry description following the proprietary Revit v2018 format (Autodesk). The format consists of a single .rvt file (binary)."@en ;
  rdfs:isDefinedBy fog: ;
  rdfs:label "as Revit format v2018 (.rvt)"@en ;
  rdfs:subPropertyOf fog:asRevit ;
.
fog:asRevit_v2019
  rdf:type owl:DatatypeProperty ;
  rdf:type owl:FunctionalProperty ;
  dbp:extension ".rvt" ;
  rdfs:comment "The datatype relation pointing to a geometry description following the proprietary Revit v2019 format (Autodesk). The format consists of a single .rvt file (binary)."@en ;
  rdfs:isDefinedBy fog: ;
  rdfs:label "as Revit format v2019 (.rvt)"@en ;
  rdfs:subPropertyOf fog:asRevit ;
.
fog:asRevit_v2020
  rdf:type owl:DatatypeProperty ;
  rdf:type owl:FunctionalProperty ;
  dbp:extension ".rvt" ;
  rdfs:comment "The datatype relation pointing to a geometry description following the proprietary Revit v2020 format (Autodesk). The format consists of a single .rvt file (binary)."@en ;
  rdfs:isDefinedBy fog: ;
  rdfs:label "as Revit format v2020 (.rvt)"@en ;
  rdfs:subPropertyOf fog:asRevit ;
.
fog:asRhino
  rdf:type owl:DatatypeProperty ;
  rdf:type owl:FunctionalProperty ;
  dbp:extension ".3dm" ;
  rdfs:comment "The datatype relation pointing to a geometry description following the proprietary Rhinoceros format (McNeel). The format consists of a single .3dm file (binary). It is strongly adviced to use the more specific subproperties (e.g. fog:asRhino_v6)"@en ;
  rdfs:isDefinedBy fog: ;
  rdfs:label "as Rhino format"@en ;
  rdfs:seeAlso wd:Q28919152 ;
  rdfs:subPropertyOf omg:hasSimpleGeometryDescription ;
.
fog:asRhino_v5
  rdf:type owl:DatatypeProperty ;
  rdf:type owl:FunctionalProperty ;
  dbp:extension ".3dm" ;
  rdfs:comment "The datatype relation pointing to a geometry description following the proprietary Rhinoceros format v5 (McNeel). The format consists of a single .3dm file (binary)."@en ;
  rdfs:isDefinedBy fog: ;
  rdfs:label "as Rhino format v5 (.3dm)"@en ;
  rdfs:seeAlso wd:Q29945416 ;
  rdfs:subPropertyOf fog:asRhino ;
.
fog:asRhino_v6
  rdf:type owl:DatatypeProperty ;
  rdf:type owl:FunctionalProperty ;
  dbp:extension ".3dm" ;
  rdfs:comment "The datatype relation pointing to a geometry description following the proprietary Rhinoceros format v6 (McNeel). The format consists of a single .3dm file (binary)."@en ;
  rdfs:isDefinedBy fog: ;
  rdfs:label "as Rhino format v6 (.3dm)"@en ;
  rdfs:subPropertyOf fog:asRhino ;
.
fog:asSfa
  rdf:type owl:DatatypeProperty ;
  rdf:type owl:FunctionalProperty ;
  rdfs:comment "The datatype relation pointing to a geometry description following the open Simple Feature Access (SFA) standard developed by the OGC and ISO. The format consists of a single .wkt (text-based) or .wkb (binary) file. It is strongly adviced to use the more specific subsubproperties (e.g. fog:asSfa_v2-wkt)."@en ;
  rdfs:isDefinedBy fog: ;
  rdfs:label "as Simple Feature Access geometry format"@en ;
  rdfs:seeAlso wd:Q365034 ;
  rdfs:seeAlso wd:Q4018860 ;
  rdfs:subPropertyOf omg:hasSimpleGeometryDescription ;
.
fog:asSfa_v1
  rdf:type owl:DatatypeProperty ;
  rdf:type owl:FunctionalProperty ;
  rdfs:comment "The datatype relation pointing to a geometry description following the open Simple Feature Access (SFA) v1 standard developed by the OGC. The format is text-based. It is strongly adviced to use the more specific subproperties (e.g. fog:asSfa_v1-wkt). Note that this standard is now considered depreciated in favor of SFA v2."@en ;
  rdfs:isDefinedBy fog: ;
  rdfs:label "as Simple Feature Access v1 format"@en ;
  rdfs:seeAlso <http://portal.opengeospatial.org/files/?artifact_id=999> ;
  rdfs:seeAlso <http://www.geoapi.org/3.0/javadoc/org/opengis/referencing/doc-files/WKT.html> ;
  rdfs:subPropertyOf fog:asSfa ;
.
fog:asSfa_v1-wkt
  rdf:type owl:DatatypeProperty ;
  rdf:type owl:FunctionalProperty ;
  rdfs:comment "The datatype relation pointing to a Well Know Text (WKT) geometry following the open Simple Feature Access (SFA) v1 standard developed by the OGC. The format is text-based. Note that the SFA v1 standard is now considered depreciated in favor of SFA v2. Note that this property is disjoint with geo:asWKT because of the more strict domain and range restrictions in GeoSPARQL."@en ;
  rdfs:isDefinedBy fog: ;
  rdfs:label "as Well Known Text SFA v1 geometry"@en ;
  rdfs:subPropertyOf fog:asSfa_v1 ;
  owl:propertyDisjointWith geo:asWKT ;
.
fog:asSfa_v2
  rdf:type owl:DatatypeProperty ;
  rdf:type owl:FunctionalProperty ;
  rdfs:comment "The datatype relation pointing to a geometry description following the open Simple Feature Access (SFA) v2 standard developed by the OGC and ISO. The format is either text-based (WKT) or binary (WKB). It is strongly adviced to use the more specific subproperties (e.g. fog:asSfa_v2-wkt)."@en ;
  rdfs:isDefinedBy fog: ;
  rdfs:label "as Simple Feature Access v2 format"@en ;
  rdfs:seeAlso <http://portal.opengeospatial.org/files/?artifact_id=25355> ;
  rdfs:subPropertyOf fog:asSfa ;
.
fog:asSfa_v2-wkb
  rdf:type owl:DatatypeProperty ;
  rdf:type owl:FunctionalProperty ;
  rdfs:comment "The datatype relation pointing to a Well Know Binary (WKB) geometry following the open Simple Feature Access (SFA) v2 standard developed by the OGC and ISO."@en ;
  rdfs:isDefinedBy fog: ;
  rdfs:label "as Well Known Binary SFA v2 geometry"@en ;
  rdfs:subPropertyOf fog:asSfa_v2 ;
.
fog:asSfa_v2-wkt
  rdf:type owl:DatatypeProperty ;
  rdf:type owl:FunctionalProperty ;
  rdfs:comment "The datatype relation pointing to a Well Know Text (WKT) geometry following the open Simple Feature Access (SFA) v2 standard developed by the OGC and ISO. The format is text-based. Note that this property is disjoint with geo:asWKT because of the more strict domain and range restrictions in GeoSPARQL."@en ;
  rdfs:isDefinedBy fog: ;
  rdfs:label "as Well Known Text SFA v2 geometry"@en ;
  rdfs:seeAlso <http://docs.opengeospatial.org/is/12-063r5/12-063r5.html> ;
  rdfs:subPropertyOf fog:asSfa_v2 ;
  owl:propertyDisjointWith geo:asWKT ;
.
fog:asShapefile
  rdf:type owl:DatatypeProperty ;
  rdfs:comment "The datatype relation pointing to a geometry description following the open Shapefile format developed by ESRI. The format consists of multiple files, including as a minimum the geometry (.shp), the index of the feature geometry (.shx) and attribute information of features (.dbf). These three files are binary, while others can be text-based (e.g. the .prj file). It is strongly adviced to use the more specific subsubproperties (e.g. fog:asShapefile-shp). Note that no file format version is provided by ESRI and that the format is expected to be stable."@en ;
  rdfs:isDefinedBy fog: ;
  rdfs:label "as Shapefile format"@en ;
  rdfs:seeAlso dbr:Shapefile ;
  rdfs:seeAlso <https://www.esri.com/library/whitepapers/pdfs/shapefile.pdf> ;
  rdfs:seeAlso wd:Q278934 ;
  rdfs:subPropertyOf omg:hasSimpleGeometryDescription ;
.
fog:asShapefile-dbf
  rdf:type owl:DatatypeProperty ;
  rdf:type owl:FunctionalProperty ;
  dbp:extension ".dbf" ;
  dcterms:requires "fog:asShapefile-shp" ;
  dcterms:requires "fog:asShapefile-shx" ;
  rdfs:comment "The datatype relation pointing to a dBASE table file (.dbf) following the open Shapefile format developed by ESRI. This file contains the attributes of each shape. The Shapefile format consists of multiple files, including as a minimum the geometry (.shp), the index of the feature geometry (.shx) and attribute information of features (.dbf). These three files are binary, while others can be text-based (e.g. the .prj file)."@en ;
  rdfs:isDefinedBy fog: ;
  rdfs:label "as Shapefile dBASE table (.dbf)"@en ;
  rdfs:seeAlso wd:Q27487130 ;
  rdfs:subPropertyOf fog:asShapefile ;
.
fog:asShapefile-prj
  rdf:type owl:DatatypeProperty ;
  rdf:type owl:FunctionalProperty ;
  dbp:extension ".prj" ;
  dcterms:requires "fog:asShapefile-dbf" ;
  dcterms:requires "fog:asShapefile-shp" ;
  dcterms:requires "fog:asShapefile-shx" ;
  rdfs:comment "The datatype relation pointing to a projection format file (.prj) following the open Shapefile format developed by ESRI. This file contains the the coordinate system and projection information of the shapes. The Shapefile format consists of multiple files, including as a minimum the geometry (.shp), the index of the feature geometry (.shx) and attribute information of features (.dbf). These three files are binary, while others can be text-based (e.g. the .prj file)."@en ;
  rdfs:isDefinedBy fog: ;
  rdfs:label "as Shapefile projections file (.prj)" ;
  rdfs:subPropertyOf fog:asShapefile ;
.
fog:asShapefile-shp
  rdf:type owl:DatatypeProperty ;
  rdf:type owl:FunctionalProperty ;
  dbp:extension ".shp" ;
  dcterms:requires "fog:asShapefile-dbf" ;
  dcterms:requires "fog:asShapefile-shx" ;
  rdfs:comment "The datatype relation pointing to a geometry file (.shp) following the open Shapefile format developed by ESRI. This file contains the geometry of the shape. The Shapefile format consists of multiple files, including as a minimum the geometry (.shp), the index of the feature geometry (.shx) and attribute information of features (.dbf). These three files are binary, while others can be text-based (e.g. the .prj file)."@en ;
  rdfs:isDefinedBy fog: ;
  rdfs:label "as Shapefile geometry (.shp)" ;
  rdfs:seeAlso wd:Q27486884 ;
  rdfs:subPropertyOf fog:asShapefile ;
.
fog:asShapefile-shx
  rdf:type owl:DatatypeProperty ;
  rdf:type owl:FunctionalProperty ;
  dbp:extension ".shx" ;
  dcterms:requires "fog:asShapefile-dbf" ;
  dcterms:requires "fog:asShapefile-shp" ;
  rdfs:comment "The datatype relation pointing to a shape index format file (.shx) following the open Shapefile format developed by ESRI. This file contains the positional index of the geometry. The Shapefile format consists of multiple files, including as a minimum the geometry (.shp), the index of the feature geometry (.shx) and attribute information of features (.dbf). These three files are binary, while others can be text-based (e.g. the .prj file)."@en ;
  rdfs:isDefinedBy fog: ;
  rdfs:label "as Shapefile geometry index (.shx)" ;
  rdfs:seeAlso wd:Q27487109 ;
  rdfs:subPropertyOf fog:asShapefile ;
.
fog:asSketchUp
  rdf:type owl:DatatypeProperty ;
  rdf:type owl:FunctionalProperty ;
  dbp:extension ".skp" ;
  rdfs:comment "The datatype relation pointing to a geometry description following the proprietary SketchUp format (Trimble). The format consists of a single .skp file (binary). It is strongly adviced to use the more specific subproperties (e.g. fog:asSketchUp_v2019)"@en ;
  rdfs:isDefinedBy fog: ;
  rdfs:label "as SketchUp format"@en ;
  rdfs:seeAlso wd:Q28975658 ;
  rdfs:subPropertyOf omg:hasSimpleGeometryDescription ;
.
fog:asSketchUp_v2017
  rdf:type owl:DatatypeProperty ;
  rdf:type owl:FunctionalProperty ;
  dbp:extension ".skp" ;
  rdfs:comment "The datatype relation pointing to a geometry description following the proprietary SketchUp v2017 format (Trimble). The format consists of a single .skp file (binary)."@en ;
  rdfs:isDefinedBy fog: ;
  rdfs:label "as SketchUp format v2017 (.skp)"@en ;
  rdfs:subPropertyOf fog:asSketchUp ;
.
fog:asSketchUp_v2018
  rdf:type owl:DatatypeProperty ;
  rdf:type owl:FunctionalProperty ;
  dbp:extension ".skp" ;
  rdfs:comment "The datatype relation pointing to a geometry description following the proprietary SketchUp v2018 format (Trimble). The format consists of a single .skp file (binary)."@en ;
  rdfs:isDefinedBy fog: ;
  rdfs:label "as SketchUp format v2018 (.skp)"@en ;
  rdfs:subPropertyOf fog:asSketchUp ;
.
fog:asSketchUp_v2019
  rdf:type owl:DatatypeProperty ;
  rdf:type owl:FunctionalProperty ;
  dbp:extension ".skp" ;
  rdfs:comment "The datatype relation pointing to a geometry description following the proprietary SketchUp v2019 format (Trimble). The format consists of a single .skp file (binary)."@en ;
  rdfs:isDefinedBy fog: ;
  rdfs:label "as SketchUp format v2019 (.skp)"@en ;
  rdfs:subPropertyOf fog:asSketchUp ;
.
fog:asStep
  rdf:type owl:DatatypeProperty ;
  rdf:type owl:FunctionalProperty ;
  dbp:extension ".step" ;
  dbp:extension ".stp" ;
  rdfs:comment "The datatype relation pointing to a geometry description following the STEP Physical File Format (SPFF) format which was developed by ISO. The format consists of a single .step file which is text-based. It is strongly adviced to use more specific subproperties."@en ;
  rdfs:isDefinedBy fog: ;
  rdfs:label "as SPFF file (.step)"@en ;
  rdfs:seeAlso wd:Q3509055 ;
  rdfs:subPropertyOf omg:hasSimpleGeometryDescription ;
.
fog:asStep_ap214
  rdf:type owl:DatatypeProperty ;
  rdf:type owl:FunctionalProperty ;
  dbp:extension ".step" ;
  dbp:extension ".stp" ;
  rdfs:comment "The datatype relation pointing to a geometry description following the STEP Physical File Format (SPFF) format which was developed by ISO. The format consists of a single .step file which is text-based. The STEP file is structured according to the Application Profile (AP) 214 - Core data for automative mechanical design processes."@en ;
  rdfs:isDefinedBy fog: ;
  rdfs:label "as STEP SPFF file (AP214)"@en ;
  rdfs:subPropertyOf fog:asStep ;
.
fog:asStep_ap242
  rdf:type owl:DatatypeProperty ;
  rdf:type owl:FunctionalProperty ;
  dbp:extension ".step" ;
  dbp:extension ".stp" ;
  rdfs:comment "The datatype relation pointing to a geometry description following the STEP Physical File Format (SPFF) format which was developed by ISO. The format consists of a single .step file which is text-based. The STEP file is structured according to the Application Profile (AP) 242 - Managed model-based 3D engineering."@en ;
  rdfs:isDefinedBy fog: ;
  rdfs:label "as STEP SPFF file (AP242)"@en ;
  rdfs:subPropertyOf fog:asStep ;
.
fog:asStl
  rdf:type owl:DatatypeProperty ;
  rdf:type owl:FunctionalProperty ;
  rdfs:comment "The datatype relation pointing to a geometry description following the STL format which was developed by 3D Systems. The format consists of a single .stl file which is either text-based or binary. It is strongly adviced to use the more specific subsubproperties (e.g. fog:asStl_v1.0-ascii)."@en ;
  rdfs:isDefinedBy fog: ;
  rdfs:label "as STL format"@en ;
  rdfs:subPropertyOf omg:hasSimpleGeometryDescription ;
.
<https://w3id.org/fog#asStl_v1.0>
  rdf:type owl:DatatypeProperty ;
  rdf:type owl:FunctionalProperty ;
  dbp:extension ".stl" ;
  rdfs:comment "The datatype relation pointing to a geometry description following the STL v1.0 format which was developed by 3D Systems. The format consists of a single .stl file which is either text-based or binary. It is strongly adviced to use the more specific subsubproperties (e.g. fog:asStl_v1.0-ascii)"@en ;
  rdfs:isDefinedBy fog: ;
  rdfs:label "as STL format v1.0"@en ;
  rdfs:seeAlso <http://paulbourke.net/dataformats/stl/> ;
  rdfs:seeAlso <https://www.iana.org/assignments/media-types/model/stl> ;
  rdfs:seeAlso wd:Q1238229 ;
  rdfs:subPropertyOf fog:asStl ;
.
<https://w3id.org/fog#asStl_v1.0-ascii>
  rdf:type owl:DatatypeProperty ;
  rdf:type owl:FunctionalProperty ;
  dbp:extension ".stl" ;
  rdfs:comment "The datatype relation pointing to a geometry description following the STL v1.0 format which was developed by 3D Systems. The format consists of a single .stl file which is text-based."@en ;
  rdfs:isDefinedBy fog: ;
  rdfs:label "as STL format v1.0 (ASCII)"@en ;
  rdfs:subPropertyOf <https://w3id.org/fog#asStl_v1.0> ;
.
<https://w3id.org/fog#asStl_v1.0-binary>
  rdf:type owl:DatatypeProperty ;
  rdf:type owl:FunctionalProperty ;
  dbp:extension ".stl" ;
  rdfs:comment "The datatype relation pointing to a geometry description following the STL v1.0 format which was developed by 3D Systems. The format consists of a single .stl file which is binary."@en ;
  rdfs:isDefinedBy fog: ;
  rdfs:label "as STL format v1.0 (binary)"@en ;
  rdfs:subPropertyOf <https://w3id.org/fog#asStl_v1.0> ;
.
fog:asSvg
  rdf:type owl:DatatypeProperty ;
  rdf:type owl:FunctionalProperty ;
  dbp:extension ".svg" ;
  rdfs:comment "The datatype relation pointing to a geometry description following the open SVG format which was developed by the W3C. The format consists of a single .svg file which is text-based. It is strongly adviced to use the more specific subsubproperties (e.g. fog:asSvg_v1.1)."@en ;
  rdfs:isDefinedBy fog: ;
  rdfs:label "as SVG format"@en ;
  rdfs:seeAlso dbr:Scalable_Vector_Graphics ;
  rdfs:seeAlso wd:Q2078 ;
  rdfs:subPropertyOf omg:hasSimpleGeometryDescription ;
.
<https://w3id.org/fog#asSvg_v1.0>
  rdf:type owl:DatatypeProperty ;
  rdf:type owl:FunctionalProperty ;
  dbp:extension ".svg" ;
  rdfs:comment "The datatype relation pointing to a geometry description following the open SVG v1.0 format which was developed by the W3C. The format consists of a single .svg file which is text-based. Note that this version (v1.0) is considered depreciated in favor of v1.1."@en ;
  rdfs:isDefinedBy fog: ;
  rdfs:label "as SVG format v1.0"@en ;
  rdfs:seeAlso <https://www.w3.org/TR/2001/REC-SVG-20010904/> ;
  rdfs:subPropertyOf fog:asSvg ;
.
<https://w3id.org/fog#asSvg_v1.1>
  rdf:type owl:DatatypeProperty ;
  rdf:type owl:FunctionalProperty ;
  dbp:extension ".svg" ;
  rdfs:comment "The datatype relation pointing to a geometry description following the open SVG v1.1 format which was developed by the W3C. The format consists of a single .svg file which is text-based."@en ;
  rdfs:isDefinedBy fog: ;
  rdfs:label "as SVG format v1.1"@en ;
  rdfs:seeAlso <https://www.w3.org/TR/SVG11/> ;
  rdfs:subPropertyOf fog:asSvg ;
.
<https://w3id.org/fog#asSvg_v2.0>
  rdf:type owl:DatatypeProperty ;
  rdf:type owl:FunctionalProperty ;
  dbp:extension ".svg" ;
  rdfs:comment "The datatype relation pointing to a geometry description following the open SVG v2.0 format which was developed by the W3C. The format consists of a single .svg file which is text-based. Note that this version (v2.0) is not yet finalized and at the moment has the status of 'W3C Candidate Recommendation'."@en ;
  rdfs:isDefinedBy fog: ;
  rdfs:label "as SVG format v2.0"@en ;
  rdfs:seeAlso <https://www.w3.org/TR/SVG2/> ;
  rdfs:subPropertyOf fog:asSvg ;
.
fog:asX3d
  rdf:type owl:DatatypeProperty ;
  rdf:type owl:FunctionalProperty ;
  rdfs:comment "The datatype relation pointing to a geometry description following the open X3D format which was developed by the Web3D. The format consists of a single file which is either binary or text-based. It is strongly adviced to use the more specific subsubproperties (e.g. fog:asX3d_v3.3_xml)."@en ;
  rdfs:isDefinedBy fog: ;
  rdfs:label "as X3D format"@en ;
  rdfs:seeAlso dbr:X3D ;
  rdfs:seeAlso <http://www.web3d.org/specifications/> ;
  rdfs:seeAlso wd:Q930428 ;
  rdfs:subPropertyOf omg:hasSimpleGeometryDescription ;
.
<https://w3id.org/fog#asX3d_v3.3>
  rdf:type owl:DatatypeProperty ;
  rdf:type owl:FunctionalProperty ;
  rdfs:comment "The datatype relation pointing to a geometry description following the open X3D v3.3 format which was developed by the Web3D. The format consists of a single file which is either binary or text-based. It is strongly adviced to use the more specific subproperties (e.g. fog:asX3d_v3.3_xml)."@en ;
  rdfs:isDefinedBy fog: ;
  rdfs:label "as X3D format v3.3"@en ;
  rdfs:subPropertyOf fog:asX3d ;
.
<https://w3id.org/fog#asX3d_v3.3-binary>
  rdf:type owl:DatatypeProperty ;
  rdf:type owl:FunctionalProperty ;
  dbp:extension ".x3db" ;
  rdfs:comment "The datatype relation pointing to a binary X3D file (.x3db) following the open X3D v3.3 format which was developed by the Web3D."@en ;
  rdfs:isDefinedBy fog: ;
  rdfs:label "as X3D v3.3 binary file (.x3db)"@en ;
  rdfs:seeAlso <http://www.web3d.org/documents/specifications/19776-3/V3.3/index.html> ;
  rdfs:subPropertyOf <https://w3id.org/fog#asX3d_v3.3> ;
.
<https://w3id.org/fog#asX3d_v3.3-vrml>
  rdf:type owl:DatatypeProperty ;
  rdf:type owl:FunctionalProperty ;
  dbp:extension ".x3dv" ;
  rdfs:comment "The datatype relation pointing to a classic VRML X3D file (.x3dv) following the open X3D v3.3 format which was developed by the Web3D. The file is text-based."@en ;
  rdfs:isDefinedBy fog: ;
  rdfs:label "as X3D v3.3 classic VRML file (.x3dv)"@en ;
  rdfs:seeAlso <http://www.web3d.org/documents/specifications/19776-2/V3.3/index.html> ;
  rdfs:seeAlso <https://www.iana.org/assignments/media-types/model/x3d-vrml> ;
  rdfs:subPropertyOf <https://w3id.org/fog#asX3d_v3.3> ;
.
<https://w3id.org/fog#asX3d_v3.3-xml>
  rdf:type owl:DatatypeProperty ;
  rdf:type owl:FunctionalProperty ;
  dbp:extension ".x3d" ;
  rdfs:comment "The datatype relation pointing to a regular X3D file (.x3d) following the open X3D v3.3 format which was developed by the Web3D. The file is text-based."@en ;
  rdfs:isDefinedBy fog: ;
  rdfs:label "as X3D v3.3 XML file (.x3d)"@en ;
  rdfs:seeAlso <http://www.web3d.org/documents/specifications/19776-1/V3.3/index.html> ;
  rdfs:seeAlso <https://www.iana.org/assignments/media-types/model/x3d+xml> ;
  rdfs:subPropertyOf <https://w3id.org/fog#asX3d_v3.3> ;
.
fog:hasIfcId
  rdf:type owl:DatatypeProperty ;
  rdfs:comment "The property links to a string containing an IFC (Industry Foundation Classes) identifier. Use any of the subproperties to be more specific regarding the type of ID."@en ;
  rdfs:label "an IFC id"@en ;
  rdfs:subPropertyOf omg:hasReferencedGeometryId ;
.
fog:hasIfcId-guid
  rdf:type owl:DatatypeProperty ;
  rdfs:comment "The property links to a string containing an IFC GUID as identifier."@en ;
  rdfs:label "an IFC GUID"@en ;
  rdfs:subPropertyOf fog:hasIfcId ;
.
fog:hasObjId
  rdf:type owl:DatatypeProperty ;
  rdfs:comment "The property links to a string containing a OBJ identifier. Use any of the subproperties to be more specific regarding the type of ID."@en ;
  rdfs:label "an OBJ identifier"@en ;
  rdfs:subPropertyOf omg:hasReferencedGeometryId ;
.
fog:hasObjId-group
  rdf:type owl:DatatypeProperty ;
  rdfs:comment "The property links to a string containing an OBJ group identifier."@en ;
  rdfs:label "an OBJ group identifier"@en ;
  rdfs:subPropertyOf fog:hasObjId ;
.
fog:hasObjId-object
  rdf:type owl:DatatypeProperty ;
  rdfs:comment "The property links to a string containing an OBJ object identifier."@en ;
  rdfs:label "an OBJ object identifier"@en ;
  rdfs:subPropertyOf fog:hasObjId ;
.
fog:hasReferencedContent
  rdf:type owl:FunctionalProperty ;
  rdf:type owl:ObjectProperty ;
  rdfs:isDefinedBy fog: ;
  rdfs:label "has referenced content" ;
  rdfs:range fog:ReferencedContent ;
.
fog:hasRevitId
  rdf:type owl:DatatypeProperty ;
  rdfs:comment "The property links to a string containing a Revit identifier. Use any of the subproperties to be more specific regarding the type of ID."@en ;
  rdfs:label "a Revit identifier"@en ;
  rdfs:subPropertyOf omg:hasReferencedGeometryId ;
.
fog:hasRevitId-element
  rdf:type owl:DatatypeProperty ;
  rdfs:comment "The property links to a string containing a Revit element identifier. This is a short ID accessible directly from the Revit interface. Beware that this ID cannot be assumed unique outside the Revit project."@en ;
  rdfs:label "a Revit element identifier"@en ;
  rdfs:subPropertyOf fog:hasRevitId ;
.
fog:hasRevitId-uniqueId
  rdf:type owl:DatatypeProperty ;
  rdfs:comment "The property links to a string containing a Revit unique identifier (UUID). According to the Autodesk specifications, it is in fact a GUID concatenated with 8 additional hexadecimal characters  corresponding to the Revit element ID."@en ;
  rdfs:label "a Revit unique identifier (UUID)"@en ;
  rdfs:subPropertyOf fog:hasRevitId ;
.
fog:hasRhinoId
  rdf:type owl:DatatypeProperty ;
  rdfs:comment "The property links to a string containing a Rhinoceros identifier. Use any of the subproperties to be more specific regarding the type of ID."@en ;
  rdfs:label "a Rhinoceros identifier"@en ;
  rdfs:subPropertyOf omg:hasReferencedGeometryId ;
.
fog:hasRhinoId-object
  rdf:type owl:DatatypeProperty ;
  rdfs:comment "The property links to a string containing a Rhinoceros object identifier, i.e. a GUID."@en ;
  rdfs:label "a Rhinoceros object identifier"@en ;
  rdfs:subPropertyOf fog:hasRhinoId ;
.
<https://www.researchgate.net/profile/Anna_Wagner13>
  rdf:type foaf:Person ;
  foaf:name "Anna Wagner" ;
.
<https://www.researchgate.net/profile/Mathias_Bonduel>
  rdf:type foaf:Person ;
  foaf:name "Mathias Bonduel" ;
.
<https://www.researchgate.net/profile/Pieter_Pauwels>
  rdf:type foaf:Person ;
  foaf:name "Pieter Pauwels" ;
.